proof draft for unfolding lemma

linear_coq/LinearRule.v
@@ -1,143 +1,15 @@
 Require Import Metalib.Metatheory.
 Require Import Program.Equality.
-Require Import Rules.
+Require Import Infra.
 
 
-Module M.
-
-Inductive IsoMode := Neg | Pos.
-
-Inductive CmpMode := Lt | Eq.
-
-
-Inductive binding : Set :=
-  | bind_sub : IsoMode -> binding
-  | bind_typ : typ -> binding.
-
-Definition env := list (atom * binding).
-Definition emp := Metatheory.empty.
-Notation empty := (@nil (atom * binding)).
+Ltac specialize_x_and_L X L :=
+  repeat match goal with
+         | [H : forall _, _ \notin L -> _, Q : X \notin L |- _ ] => specialize (H _ Q); clear Q
+         | [H : forall _, _ \notin L -> _ |- _ ] => assert (X \notin L) by auto
+         end.
 
 
-Inductive WFS : env -> typ -> Prop :=
-| WFS_top : forall E, WFS E typ_top
-| WFS_nat : forall E, WFS E typ_nat
-| WFS_fvar : forall X E im,
-    binds X (bind_sub im) E ->
-    WFS E (typ_fvar X)
-| WFS_arrow : forall E A B,
-    WFS E A ->
-    WFS E B ->
-    WFS E (typ_arrow A B)
-| WFS_rec : forall L E A im,
-    (* (forall X , X \notin L -> forall im, 
-        WFS (X ~ bind_sub im ++ E) (open_tt A (typ_rcd X (open_tt A X)))) -> *)
-      (forall  X , X \notin L -> 
-        WFS (X ~ bind_sub im ++ E) (open_tt A X)) ->
-      WFS E (typ_mu A).
-
-
-Inductive wf_env : env -> Prop :=
-  | wf_env_empty :
-      wf_env empty
-  | wf_env_sub : forall (E : env) (X : atom) im,
-      wf_env E ->
-      X \notin dom E ->
-      wf_env (X ~ bind_sub im ++ E)
-  | wf_env_typ : forall (E : env) (x : atom) (T : typ),
-      wf_env E ->
-      WFS E T ->
-      x `notin` dom E ->
-      wf_env (x ~ bind_typ T ++ E).
-
-Definition flip_im (im : IsoMode) : IsoMode :=
-  match im with
-    | Neg => Pos
-    | Pos => Neg
-  end.
-
-Definition compose_cm (cm1 cm2 : CmpMode) (evs1 evs2 : atoms ) : option (CmpMode) :=
-  match cm1, cm2 with
-    | Lt, Lt => Some Lt
-    | Eq, Lt => if AtomSetImpl.is_empty evs1 then Some Lt else None
-    | Lt, Eq => if AtomSetImpl.is_empty evs2 then Some Lt else None
-    | Eq, Eq => Some Eq
-  end.
-
-
-(*
-IsoMode := + | -
-E [IsoMode] |- T1 [CmpMode] T2
-*)
-Inductive Sub : IsoMode -> CmpMode -> atoms -> env -> typ -> typ -> Prop :=
-(* 
-|- E
-----------------
-E [_]|- nat <:= nat 
-*)
-| Sa_nat: forall E im,
-    wf_env E ->
-    Sub im Eq emp E typ_nat typ_nat
-(*
-|- E
-----------------
-E [=] |- top <:= top
-*)
-| Sa_top_eq: forall E im,
-    wf_env E ->
-    Sub im Eq emp E typ_top typ_top  
-(*
-TODO: is != top necessary?, if we are going to interpret <: as no greater than
-|- E, A != top
-----------------
-E [<] |- A <:= top
-*)
-| Sa_top_lt: forall E im A,
-    wf_env E -> WFS E A -> A <> typ_top ->
-    Sub im Lt emp E A typ_top
-| Sa_fvar_pos: forall E X im,
-    wf_env E -> binds X (bind_sub im) E ->
-    Sub im Eq emp E (typ_fvar X) (typ_fvar X)
-| Sa_fvar_neg: forall E X im,
-    wf_env E -> binds X (bind_sub (flip_im im)) E ->
-    Sub im Eq (singleton X) E (typ_fvar X) (typ_fvar X)
-| Sa_arrow: forall E A1 A2 B1 B2 cm1 cm2 evs1 evs2 cm im,
-    Sub (flip_im im) cm1 evs1 E B1 A1 ->
-    Sub im cm2 evs2 E A2 B2 ->
-    compose_cm cm1 cm2 evs1 evs2 = Some cm ->
-    Sub im cm (evs1 `union` evs2) E (typ_arrow A1 A2) (typ_arrow B1 B2)
-| Sa_rec_lt: forall L A1 A2 evs E im,
-    (forall X,  X \notin L -> 
-        Sub im Lt evs (X ~ bind_sub im ++ E) (open_tt A1 X) (open_tt A2 X)) ->
-        (* implicitly indicates that X cannot be in the weak-positive set of  E,x |-  A1 <: A2 *)
-    Sub im Lt evs E (typ_mu A1) (typ_mu A2)
-| Sa_rec_eq_notin: forall L A1 A2 evs E im,
-    (forall X,  X \notin L -> 
-        Sub im Eq evs (X ~ bind_sub im ++ E) (open_tt A1 X) (open_tt A2 X)) ->
-    Sub im Eq evs E (typ_mu A1) (typ_mu A2)
-(* | Sa_rec_eq_in: forall L A1 A2 evs E im,
-    (forall X,  X \notin L -> 
-      exists evs', (evs `union` {{X}}) [=] evs' /\
-        Sub im Eq evs' (X ~ bind_sub im ++ E) (open_tt A1 X) (open_tt A2 X)) ->
-    Sub im Eq (evs `union` fv_tt A1) E (typ_mu A1) (typ_mu A2) *)
-| Sa_rec_eq_in: forall L A1 A2 evs E im,
-    (forall X,  X \notin L -> 
-        Sub im Eq (add X evs) (X ~ bind_sub im ++ E) (open_tt A1 X) (open_tt A2 X)) ->
-    Sub im Eq (evs `union` fv_tt A1) E (typ_mu A1) (typ_mu A2)
-| Sa_evs_proper: forall im cm evs evs' E A1 A2,
-    Sub im cm evs E A1 A2 ->
-    evs [=] evs' ->
-    Sub im cm evs' E A1 A2
-.
-
-#[global] Hint Constructors Sub wf_env WFS : core.
-
-
-(* 
-
-mu a. Top -> (mu b. b -> a) is not subtype of mu a. a -> (mu b. b -> a)
-
-*)
 #[global]
 Instance sub_m : Proper (eq ==> eq ==> AtomSetImpl.Equal ==> eq ==> eq ==> eq ==> iff) Sub.
 Proof with auto.
@@ -270,8 +142,8 @@ Proof with auto.
     subst...
 Qed.
 
-Theorem sub_regular: forall E im evs A B,
-  Sub im Eq evs E A B -> wf_env E /\ WFS E A /\ WFS E B.
+Theorem sub_regular: forall E im cm evs A B,
+  Sub im cm evs E A B -> wf_env E /\ WFS E A /\ WFS E B.
 Proof with auto.
   intros. induction H...
   - split... split... 
@@ -619,8 +491,6 @@ Proof with auto.
   - apply type_mu with (L:=L)...
 Qed.
 
-End M.
-
 
 Ltac gather_atoms ::=
   let A := gather_atoms_with (fun x : atoms => x) in
@@ -629,37 +499,36 @@ Ltac gather_atoms ::=
   let C := gather_atoms_with (fun x : list (var * typ) => dom x) in
   let D := gather_atoms_with (fun x : exp => fv_exp x) in
   let F := gather_atoms_with (fun x : env => dom x) in
-  let G := gather_atoms_with (fun x : M.env => dom x) in
-  constr:(A `union` B `union`  E \u C \u D \u F \u G).
+  constr:(A `union` B `union`  E \u C \u D \u F).
 
 
 
 Theorem Msub_refl: forall E im A,
-    M.wf_env E -> type A -> M.WFS E A -> exists evs, M.Sub im M.Eq evs E A A.
+    wf_env E -> type A -> WFS E A -> exists evs, Sub im Eq evs E A A.
 Proof with auto.
   intros. generalize dependent im. generalize dependent E. induction H0;intros...
-  - exists M.emp...
-  - exists M.emp...
+  - exists emp...
+  - exists emp...
   - inversion H1;subst. destruct im, im0.
-    + exists M.emp...
+    + exists emp...
     + exists (singleton X)...
     + exists (singleton X)...
-    + exists M.emp...
-  - inversion H1;subst. destruct IHtype1 with (im:=M.flip_im im) (E:=E) as [evs1 ?], IHtype2 with (im:=im) (E:=E) as [evs2 ?]...
+    + exists emp...
+  - inversion H1;subst. destruct IHtype1 with (im:=flip_im im) (E:=E) as [evs1 ?], IHtype2 with (im:=im) (E:=E) as [evs2 ?]...
     exists (union evs1 evs2)...
-    apply M.Sa_arrow with (cm1:=M.Eq) (cm2:=M.Eq)...
+    apply Sa_arrow with (cm1:=Eq) (cm2:=Eq)...
   - 
     inversion H2;subst.
     pick_fresh X. specialize_x_and_L X L. specialize_x_and_L X L0.
     (* need to decide whether X is in evs of (open_tt T X), so we need replacing_var lemma *)
-    destruct H0 with (im:=im) (E:=X ~ M.bind_sub im ++ E) as [evs1 ?]...
-    { rewrite_alist (nil ++ X ~ M.bind_sub im ++ E). apply M.WFS_im_inv with (im1:=im0)... }
+    destruct H0 with (im:=im) (E:=X ~ bind_sub im ++ E) as [evs1 ?]...
+    { rewrite_alist (nil ++ X ~ bind_sub im ++ E). apply WFS_im_inv with (im1:=im0)... }
     exists (if AtomSetImpl.mem X evs1 then (remove X evs1) \u fv_tt T else evs1)...
     destruct (AtomSetImpl.mem X evs1) eqn:Evs1.
     + apply mem_iff in Evs1.
-      apply M.Sa_rec_eq_in with (L:=L \u {{X}} \u evs1 \u dom E).
+      apply Sa_rec_eq_in with (L:=L \u {{X}} \u evs1 \u dom E).
       intros.
-      rewrite_alist (nil ++ (X0 ~ M.bind_sub im) ++ E).
+      rewrite_alist (nil ++ (X0 ~ bind_sub im) ++ E).
       replace (add X0 (remove X evs1)) with 
       (if AtomSetImpl.mem X evs1 then add X0 (remove X evs1) else evs1)...
       2:{ destruct (AtomSetImpl.mem X evs1) eqn:Evs2;
@@ -668,12 +537,12 @@ Proof with auto.
           | [ H: AtomSetImpl.mem _ _ = false |- _ ] => apply not_mem_iff in H end;
           try solve [exfalso;auto];
           try fsetdec. }
-      rewrite_alist (nil ++ (X0 ~ M.bind_sub im) ++ E).
-      apply M.sub_replacing_var... constructor...
+      rewrite_alist (nil ++ (X0 ~ bind_sub im) ++ E).
+      apply sub_replacing_var... constructor...
     + apply not_mem_iff in Evs1.
-      apply M.Sa_rec_eq_notin with (L:=L \u {{X}} \u evs1 \u dom E).
+      apply Sa_rec_eq_notin with (L:=L \u {{X}} \u evs1 \u dom E).
       intros.
-      rewrite_alist (nil ++ (X0 ~ M.bind_sub im) ++ E).
+      rewrite_alist (nil ++ (X0 ~ bind_sub im) ++ E).
       replace (evs1) with 
       (if AtomSetImpl.mem X evs1 then add X0 (remove X evs1) else evs1)...
       2:{ destruct (AtomSetImpl.mem X evs1) eqn:Evs2;
@@ -682,83 +551,13 @@ Proof with auto.
           | [ H: AtomSetImpl.mem _ _ = false |- _ ] => apply not_mem_iff in H end;
           try solve [exfalso;auto];
           try fsetdec. }
-      apply M.sub_replacing_var... constructor...
+      apply sub_replacing_var... constructor...
 Qed.
 
-Definition drop_mode (b: M.binding) : binding := match b with
-| M.bind_sub _ => bind_sub
-| M.bind_typ t => bind_typ t
-end.
-
-Definition env_of (E: M.env) := map drop_mode E.
-
-Lemma binds_M_to_binds: forall im X E,
-  binds X (M.bind_sub im) E ->
-  binds X (bind_sub) (env_of E).
-Proof with auto.
-  intros.
-  induction E...
-  { destruct a. inversion H;subst;simpl in *...
-      inversion H0;subst... }
-Qed.
-
-Theorem WFS_M_WFA: forall E A, M.WFS E A -> WFA (env_of E) A.
-Proof with auto.
-  intros. induction H;simpl in *...
-  - apply WFA_fvar. apply binds_M_to_binds in H...
-  - apply WFA_rec with (L:=L)...
-Qed.
-
-Lemma env_of_wf_env: forall E, M.wf_env E -> wf_env (env_of E).
-Proof with auto.
-  intros. induction H;simpl in *...
-  - constructor... unfold env_of. rewrite dom_map...
-  - constructor... { apply WFS_M_WFA in H0. apply soundness_wfa in H0... }
-    unfold env_of. rewrite dom_map...
-Qed.
-
-#[global]
-Hint Resolve env_of_wf_env WFS_M_WFA soundness_wfa M.WFS_type : core.
-
-
-Lemma open_tt_fresh_eq_inv: forall A B X,
-  X `notin` fv_tt A ->
-  X `notin` fv_tt B ->
-  open_tt A X = open_tt B X ->
-  A = B.
-Proof with auto.
-  unfold open_tt. generalize 0.
-  intros. unfold open_tt in H1. generalize dependent B.
-  generalize dependent n.
-  induction A;intros...
-  - induction B;inversion H1...
-    destruct (n == n0);inversion H3.
-  - induction B;inversion H1...
-    destruct (n == n0);inversion H3.
-  - simpl in H1.
-    destruct (n0 == n).
-    + induction B;inversion H1...
-      { destruct (n0 == n1);inversion H1;subst...
-        inversion H3. }
-      { simpl in H1. subst. exfalso... apply H0. simpl... }
-    + induction B;inversion H1...
-      { destruct (n0 == n2);inversion H1;subst...
-        inversion H3. }
-  - induction B;inversion H1...
-    destruct (n == n0);inversion H3.
-    simpl in H1. subst. exfalso... apply H. simpl...
-  - induction B;inversion H1...
-    destruct (n == n0);inversion H3.
-    rewrite IHA with (n:=S n) (B:=B)...
-  - induction B;inversion H1...
-    destruct (n == n0);inversion H3. simpl in H, H0.
-    rewrite IHA1 with (n:=n) (B:=B1)...
-    rewrite IHA2 with (n:=n) (B:=B2)...
-Qed.
 
 
 Theorem Msub_refl_inv: forall E im A B evs,
-    M.Sub im M.Eq evs E A B -> A = B.
+    Sub im Eq evs E A B -> A = B.
 Proof with auto.
   intros. dependent induction H...
   - destruct cm1, cm2; try solve [ simpl in H1;
@@ -772,148 +571,8 @@ Proof with auto.
     specialize (H0 eq_refl). apply open_tt_fresh_eq_inv in H0... subst...
 Qed.
 
-
-Definition mode_of (im: M.IsoMode) : Mode := match im with
-| M.Pos => Pos | M.Neg => Neg end.
-
-Lemma mode_of_flip: forall im, mode_of (M.flip_im im) = flip (mode_of im).
-Proof. destruct im;auto. Qed.
-
-
-Theorem soundness_posvar: forall E im cm evs A B,
-  M.Sub im cm evs E A B -> forall X, X `notin` evs -> 
-    (binds X (M.bind_sub im) E ->  posvar Pos X A B) /\
-    (binds X (M.bind_sub (M.flip_im im)) E ->  posvar Neg X A B).
-Proof with auto.
-  intros. generalize dependent X.
-  induction H;intros...
-  - split;intros. 
-    + constructor. apply M.WFS_type in H0...
-    + constructor. apply M.WFS_type in H0...
-  - split;intros.
-    + destruct (X == X0).
-      2:{ apply pos_fvar_y... }
-      subst. apply pos_fvar_x.
-    + destruct (X == X0).
-      2:{ apply pos_fvar_y... }
-      subst. apply M.uniq_from_wf_env in H.
-      pose proof binds_unique _ _ _ _ _ H0 H2 H.
-      inversion H3. destruct im;inversion H5.
-  - destruct IHSub1 with (X:=X)... destruct IHSub2 with (X:=X)...
-    split;intros.
-    + constructor... apply H4. destruct im...
-    + constructor...
-  - 
-    (* rec lt *)
-    split;intros.
-    + apply pos_rec with (L:=L \u evs)...
-      * intros. specialize_x_and_L Y L... destruct H0 with (X:=X)...
-      * intros. specialize_x_and_L Y L... destruct H0 with (X:=Y)...
-    + apply pos_rec with (L:=L \u evs)...
-      * intros. specialize_x_and_L Y L... destruct H0 with (X:=X)...
-      * intros. specialize_x_and_L Y L... destruct H0 with (X:=Y)...
-  - 
-    (* rec eq notin *)
-    split;intros.
-    + apply pos_rec with (L:=L \u evs)...
-      * intros. specialize_x_and_L Y L... destruct H0 with (X:=X)...
-      * intros. specialize_x_and_L Y L... destruct H0 with (X:=Y)...
-    + apply pos_rec with (L:=L \u evs)...
-      * intros. specialize_x_and_L Y L... destruct H0 with (X:=X)...
-      * intros. specialize_x_and_L Y L... destruct H0 with (X:=Y)...
-  -
-    (* rec eq in *)
-    assert (typ_mu A1 = typ_mu A2).
-    { assert (M.Sub im M.Eq (evs `union` fv_tt A1) E (typ_mu A1) (typ_mu A2))...
-      { apply M.Sa_rec_eq_in with (L:=L)... }
-      apply Msub_refl_inv in H2... }
-    rewrite <- H2. split;intros.
-    + apply pos_rec_t with (L:=L)...
-      { intros. specialize_x_and_L Y L. apply M.sub_regular in H. destruct_hypos. apply M.WFS_type in H5... }
-    + apply pos_rec_t with (L:=L)...
-      { intros. specialize_x_and_L Y L. apply M.sub_regular in H. destruct_hypos. apply M.WFS_type in H5... }
-  -
-    rewrite <- H0 in H1...
-Qed.
-
-
-Theorem soundness_posvar_fresh: forall E im im' cm evs A B,
-  M.Sub im cm evs E A B -> forall X, X `notin` evs \u dom E -> 
-    posvar im' X A B.
-Proof with auto.
-  intros. generalize dependent X. generalize dependent im'.
-  induction H;intros...
-  - constructor. apply M.WFS_type in H0...
-  - constructor. apply binds_In in H0. intros C. subst...
-  - 
-    (* rec lt *)
-    apply pos_rec with (L:=L \u evs)...
-    * intros. specialize_x_and_L Y L...
-      apply soundness_posvar with (X:=Y) in H...
-      destruct H...
-  - 
-    (* rec eq notin *)
-    apply pos_rec with (L:=L \u evs)...
-    * intros. specialize_x_and_L Y L...
-      apply soundness_posvar with (X:=Y) in H...
-      destruct H...
-  -
-    (* rec eq in *)
-    assert (typ_mu A1 = typ_mu A2).
-    { assert (M.Sub im M.Eq (evs `union` fv_tt A1) E (typ_mu A1) (typ_mu A2))...
-      { apply M.Sa_rec_eq_in with (L:=L)... }
-      apply Msub_refl_inv in H2... }
-    rewrite <- H2. apply pos_rec_t with (L:=L)...
-    { intros. specialize_x_and_L Y L. apply M.sub_regular in H. destruct_hypos. apply M.WFS_type in H4... }
-  -
-    rewrite <- H0 in H1...
-Qed.
-
-
-
-Theorem soundness: forall E im cm evs A B,
-  M.Sub im cm evs E A B -> sub_amber2 (env_of E) A B.
-Proof with auto.
-  intros. induction H;intros...
-  - apply binds_M_to_binds in H0...
-  - apply binds_M_to_binds in H0...
-  - 
-    (* rec lt *)
-    apply sam2_rec with (L:=L \u evs \u dom E)...
-    + intros. specialize_x_and_L X L...
-    + intros.
-      apply pos_rec with (L:=L \u dom E \u evs)...
-      * intros. specialize_x_and_L Y L...
-        apply soundness_posvar_fresh with (X:=X) (im':=Pos) in H...
-      * intros. specialize_x_and_L Y L...
-        apply soundness_posvar with (X:=Y) in H...
-        destruct H...
-  -
-    (* rec eq notin *)
-    apply sam2_rec with (L:=L \u evs \u dom E)...
-    + intros. specialize_x_and_L X L...
-    + intros.
-      apply pos_rec with (L:=L \u dom E \u evs)...
-      * intros. specialize_x_and_L Y L...
-        apply soundness_posvar_fresh with (X:=X) (im':=Pos) in H...
-      * intros. specialize_x_and_L Y L...
-        apply soundness_posvar with (X:=Y) in H...
-        destruct H...
-  -
-    (* rec eq in *)
-    apply sam2_rec with (L:=L \u evs \u dom E \u fv_tt A1)...
-    + intros. specialize_x_and_L X L...
-    + intros.
-      assert (typ_mu A1 = typ_mu A2).
-      { assert (M.Sub im M.Eq (evs `union` fv_tt A1) E (typ_mu A1) (typ_mu A2))...
-        { apply M.Sa_rec_eq_in with (L:=L)... }
-        apply Msub_refl_inv in H2... } rewrite <- H2.
-      apply pos_rec_t with (L:=L \u dom E \u evs \u fv_tt A1)...
-      { intros. specialize_x_and_L Y L. apply M.sub_regular in H. destruct_hypos. apply M.WFS_type in H4... }
-Qed.
-
 Lemma Msub_lt_not_eq: forall im evs E A B,
-  M.Sub im M.Lt evs E A B -> A <> B.
+  Sub im Lt evs E A B -> A <> B.
 Proof with auto.
   intros. dependent induction H...
   - destruct cm1.
@@ -926,110 +585,6 @@ Proof with auto.
     apply H0...
 Qed.
 
-
-Theorem posvar_false: forall E im cm evs A B,
-  M.Sub im cm evs E A B ->  forall X, X `in` evs -> 
-    (binds X (M.bind_sub im) E ->  ~ posvar Pos X A B) /\
-    (binds X (M.bind_sub (M.flip_im im)) E ->  ~ posvar Neg X A B).
-    (* ~ posvar (mode_of im) X A B. *)
-Proof with auto.
-  intros. generalize dependent X.
-  induction H;intros...
-  (* if induction on H, then for var case we cannot get IH for evs1 evs2 *)
-  - fsetdec.
-  - fsetdec.
-  - fsetdec.
-  - fsetdec.
-  - assert (X0 = X) by fsetdec. subst. split;intros.
-    + apply M.uniq_from_wf_env in H.
-      pose proof binds_unique _ _ _ _ _ H0 H2 H.
-      destruct im; inversion H3.
-    + intros C. inversion C;subst...
-  - apply union_iff in H2.
-    destruct H2.
-    + specialize (IHSub1 _ H2).
-      destruct IHSub1. split;intros.
-      * intros C. inversion C;subst. apply H4... destruct im...
-      * intros C. inversion C;subst. apply H3...
-    + specialize (IHSub2 _ H2).
-      destruct IHSub2. split;intros.
-      * intros C. inversion C;subst. apply H3...
-      * intros C. inversion C;subst. apply H4...
-  -
-    (* rec lt *)
-    split;intros.
-    + intros C. inversion C;subst.
-      { (* rec posvar *)
-        pick_fresh Y. specialize_x_and_L Y L. specialize_x_and_L Y (union L0 (singleton X)).
-        specialize (H0 X H1).
-        destruct H0... apply H0... }
-      { (* rec self *)
-        pick_fresh Y. specialize_x_and_L Y L.
-        apply Msub_lt_not_eq in H...
-      }
-    + intros C. inversion C;subst.
-      { (* rec posvar *)
-        pick_fresh Y. specialize_x_and_L Y L. specialize_x_and_L Y (union L0 (singleton X)).
-        specialize (H0 X H1).
-        destruct H0... apply H3... }
-      { (* rec self *)
-        pick_fresh Y. specialize_x_and_L Y L.
-        apply Msub_lt_not_eq in H...
-      }
-  -
-    (* rec eq notin *)
-    split;intros.
-    + intros C. inversion C;subst.
-      { (* rec posvar *)
-        pick_fresh Y. specialize_x_and_L Y L. specialize_x_and_L Y (union L0 (singleton X)).
-        destruct H0 with (X:=X)... apply H3... }
-      { (* rec self *)
-        pick_fresh Y. specialize_x_and_L Y L.
-        apply M.sub_evs_fv in H. destruct_hypos.
-        apply H in H1. apply in_open1 in H1. simpl in H1. destruct H1... fsetdec. }
-    + intros C. inversion C;subst.    
-      { (* rec posvar *)
-        pick_fresh Y. specialize_x_and_L Y L. specialize_x_and_L Y (union L0 (singleton X)).
-        destruct H0 with (X:=X)... apply H4... }
-      { (* rec self *)
-        pick_fresh Y. specialize_x_and_L Y L.
-        apply M.sub_evs_fv in H. destruct_hypos.
-        apply H in H1. apply in_open1 in H1. simpl in H1. destruct H1... fsetdec. }
-  -
-    split;intros.
-    + intros C. inversion C;subst.
-      { (* rec posvar *)
-        pick_fresh Y.
-        apply union_iff in H1. destruct H1.
-        + specialize_x_and_L Y L. specialize_x_and_L Y (union L0 (singleton X)).
-          destruct H0 with (X:=X)... apply H3...
-        + specialize_x_and_L Y L. specialize_x_and_L Y (union L0 (singleton X)).
-          destruct H0 with (X:=Y)... (* <--- key of the proof *)
-          apply H3... }
-      { (* rec self *)
-        apply union_iff in H1. destruct H1. 2:{ fsetdec. }
-        pick_fresh Y. specialize_x_and_L Y L.
-        apply M.sub_evs_fv in H. destruct_hypos.
-        apply (@KeySetProperties.subset_add_2 evs evs Y) in H1;try reflexivity.
-        apply H in H1. apply in_open1 in H1. simpl in H1. destruct H1... fsetdec. }
-    + intros C. inversion C;subst.    
-      { (* rec posvar *)
-        pick_fresh Y.
-        apply union_iff in H1. destruct H1.
-        + specialize_x_and_L Y L. specialize_x_and_L Y (union L0 (singleton X)).
-          destruct H0 with (X:=X)... apply H4...
-        + specialize_x_and_L Y L. specialize_x_and_L Y (union L0 (singleton X)).
-          destruct H0 with (X:=Y)... (* <--- key of the proof *)
-          apply H3... }
-      { (* rec self *)
-        apply union_iff in H1. destruct H1. 2:{ fsetdec. }
-        pick_fresh Y. specialize_x_and_L Y L.
-        apply M.sub_evs_fv in H. destruct_hypos.
-        apply (@KeySetProperties.subset_add_2 evs evs Y) in H1;try reflexivity.
-        apply H in H1. apply in_open1 in H1. simpl in H1. destruct H1... fsetdec. }
-  -
-    rewrite <- H0 in H1...
-Qed.
 
 Lemma is_not_empty_iff: forall s,
   AtomSetImpl.is_empty s = false <-> ~ AtomSetImpl.Empty s .
@@ -1047,411 +602,64 @@ Proof with auto.
   - apply AtomSetImpl.choose_2 in E... congruence.
 Qed.
 
-
-Inductive is_Menv : M.env -> env -> Prop :=
-  | is_Menv_nil: is_Menv nil nil
-  | is_Menv_sub_pos: forall E' E X,
-      is_Menv E' E ->
-      is_Menv ((X, M.bind_sub M.Pos) :: E') ((X, bind_sub) :: E)
-  | is_Menv_sub_neg: forall E' E X,
-      is_Menv E' E ->
-      is_Menv ((X, M.bind_sub M.Neg) :: E') ((X, bind_sub) :: E)
-  | is_Menv_typ: forall E' E X T,
-      is_Menv E' E ->
-      is_Menv ((X, M.bind_typ T) :: E') ((X, bind_typ T) :: E).
-
-(* 
-
-cannot make useof posvar_false if expressed as exists
-
-
-
-Theorem completeness: forall E A B,
-  (* is_Menv E E' -> *)
-  sub_amber2 (env_of E) A B -> forall im,
-  (exists evs cm, M.Sub im cm evs E A B /\ 
-  (forall X, X \in evs ->
-     (binds X (M.bind_sub ( im)) E -> ~ posvar Pos  X A B) /\
-     (binds X (M.bind_sub ( (M.flip_im im))) E -> ~ posvar Neg X A B))).
+Lemma generalized_unfolding_lemma:
+  forall E1 E2 C D A B X im evs,
+    wf_env (E1 ++ E2) -> X \notin fv_tt C \u fv_tt D \u dom (E1 ++ E2) ->
+    Sub im Lt evs (E1 ++ X ~ bind_sub im ++ E2) A B ->
+    Sub im Lt evs (E1 ++ E2) (subst_tt X (typ_mu C) A) (subst_tt X (typ_mu D) B).
 Proof with auto.
-  intros. dependent induction H...
-  - exists M.emp, M.Eq. split... apply M.Sa_nat... admit. intros. fsetdec.
-  - admit.
-  - assert (binds X (M.bind_sub im) E \/ binds X (M.bind_sub (M.flip_im im)) E).
-    { admit. }
-    destruct H1.
-    + exists M.emp, M.Eq. split... apply M.Sa_fvar_pos... admit. intros. fsetdec.
-    + exists {{ X }}, M.Eq. split... apply M.Sa_fvar_neg... admit. intros. assert (X0 = X) by fsetdec. subst...
-      split.
-      * intros. admit.
-      * intros. intros C. inversion C...
-      (* * intros. assert (im = M.Pos) by admit. subst. intros C. inversion C... *)
+  intros.
+  dependent induction H1;intros...
   -
-    destruct IHsub_amber2_1 with (im:=M.flip_im im) (E0:=E) as [evs1 [cm1 [IH1 IH1']]]...
-    destruct cm1.
-    + destruct IHsub_amber2_2 with (im:=im) (E0:=E) as [evs2 [cm2 [IH2 IH2']]]...
-      destruct cm2.
-      * (* lt + lt *)
-        exists (union evs1 evs2), M.Lt. split.
-        { apply M.Sa_arrow with (cm1:=M.Lt) (cm2:=M.Lt)... }
-        { intros. apply union_iff in H1. destruct H1.
-          - apply IH1' in H1... destruct H1... split;intros;intros C;inversion C;subst...
-            { apply H2... destruct im... }
-            { apply H1... }
-          - apply IH2' in H1... destruct H1... split;intros;intros C;inversion C;subst...
-            { apply H1... }
-            { apply H2... }
-        }
-      * (* lt + eq *)
-        destruct (AtomSetImpl.is_empty evs2) eqn:Eempty.
-        2:{ (* evs2 cannot be empty *)
-            apply is_not_empty_iff in Eempty. apply not_empty_has in Eempty.
-            destruct Eempty as [X Eempty].
-            pose proof posvar_false _ _ _ _ _ _ IH2 X Eempty.
-            destruct H1.
-            apply IH2' in Eempty. destruct Eempty as [IH2'1 IH2'2].
-
-    + 
-    destruct IHsub_amber2_2 with (im:=im) (E0:=E) as [evs2 [cm2 [IH2 IH2']]]...
-    exists (union evs1 evs2), (M.compose_cm cm1 cm2). split.
-    + apply M.Sa_and... admit. admit.
-    + intros. apply union_iff in H1. destruct H1.
-      * apply IH1' in H1... destruct H1...
-      * apply IH2' in H1... destruct H1...
-  
- *)
-
-Lemma is_Menv_case: forall E0 E X im,
-is_Menv E0 E -> 
-binds X bind_sub E ->
-(binds X (M.bind_sub im) E0 \/ binds X (M.bind_sub (M.flip_im im)) E0).
-Proof with auto.
-  intros.
-  induction H...
-  - analyze_binds H0.
-    + destruct im...
-    + destruct IHis_Menv...
-  - analyze_binds H0.
-    + destruct im...
-    + destruct IHis_Menv...
-  - analyze_binds H0.
-    destruct IHis_Menv...
-Qed.
-
-
-Lemma is_Menv_dom: forall E E',
-    is_Menv E E' -> dom E [=] dom E'.
-Proof with auto.
-  intros. induction H...
-  - simpl. reflexivity.
-  - simpl. rewrite IHis_Menv... reflexivity.
-  - simpl. rewrite IHis_Menv... reflexivity.
-  - simpl. rewrite IHis_Menv... reflexivity.
-Qed.
-
-Lemma is_Menv_binds: forall E E' X im,
-    is_Menv E E' -> binds X (M.bind_sub im) E -> binds X bind_sub E'.
-Proof with auto.
-  intros. induction H...
-  - inversion H0;subst... inversion H1;subst...
-  - inversion H0;subst... inversion H1;subst...
-  - inversion H0;subst... inversion H1;subst...
-Qed.
-
-Lemma MWFS_WF: forall E E' A,
-  is_Menv E E' ->
-  M.WFS E A -> WF E' A.
-Proof with auto.
-  intros. generalize dependent E'. induction H0;intros...
-  - apply is_Menv_binds with (E':=E') in H...
-  - apply WF_rec with (L:=L \u fv_tt A)...
-    + intros. specialize_x_and_L X L.
-      apply H0... destruct im; constructor...
-    + intros. specialize_x_and_L X L.
-      rewrite subst_tt_intro with (X:=X)...
-      apply subst_tt_wf;apply H0;destruct im;constructor...
-Qed.
-
-
-Lemma is_Menv_binds2: forall E E' X,
-    is_Menv E E' -> binds X bind_sub E' -> 
-    exists im, binds X (M.bind_sub im) E.
-Proof with auto.
-  intros. induction H...
-  - inversion H0...
-  - analyze_binds H0.
-    { exists M.Pos... }
-    { destruct IHis_Menv... exists x... }
-  - analyze_binds H0.
-    { exists M.Neg... }
-    { destruct IHis_Menv... exists x... }
-  - analyze_binds H0.
-    { destruct IHis_Menv... exists x... }
-Qed.
-
-Lemma MWF_WFS: forall E E' A,
-  is_Menv E E' ->
-  WF E' A -> M.WFS E A.
-Proof with auto.
-  intros. generalize dependent E. induction H0;intros...
-  - destruct (is_Menv_binds2 _ _ _ H0 H)...
-    apply M.WFS_fvar with (im:=x)...
-  - apply M.WFS_rec with (L:=L \u fv_tt A) (im:=M.Pos) ...
-    + intros. apply H0... constructor...
-Qed.
-
-
-
-Lemma Menv_wf_env: forall E E',
-    is_Menv E E' ->
-    M.wf_env E -> wf_env E'.
-Proof with auto.
-  intros.
-  induction H;intros...
-  - inversion H0;subst. constructor...
-    rewrite <- is_Menv_dom with (E:=E')...
-  - inversion H0;subst. constructor...
-    rewrite <- is_Menv_dom with (E:=E')...
-  - inversion H0;subst. constructor...
-    { apply soundness_wf. apply MWFS_WF with (E:=E')... }
-    { rewrite <- is_Menv_dom with (E:=E')... }
-Qed.
-
-
-
-Lemma is_Menv_wf_env: forall E0 E,
-is_Menv E0 E -> wf_env E -> M.wf_env E0.
-Proof with auto.
-  intros.
-  induction H...
-  - inversion H0;subst. constructor...
-    rewrite is_Menv_dom with (E:=E')...
-  - inversion H0;subst. constructor...
-    rewrite is_Menv_dom with (E:=E')...
-  - inversion H0;subst. constructor...
-    { apply completeness_wf in H5. apply MWF_WFS with (E':=E)... }
-    { rewrite is_Menv_dom with (E:=E')... }
-Qed.
-
-#[global] Hint Resolve is_Menv_wf_env : core.
-
-Lemma WFA_binds: forall E A X,
-  X `in` fv_tt A -> WF E A -> binds X bind_sub E.
-Proof with auto.
-  intros. induction H0;simpl in *;try solve [fsetdec]...
-  - assert (X = X0) by fsetdec. subst...
-  - apply union_iff in H. destruct H...
-  - pick_fresh Y. specialize_x_and_L Y L.
-    destruct H1...
-    { apply in_open... }
-    inversion H1;subst... exfalso...
-Qed.
-
-Lemma uniq_from_wf_env: forall E,
-    wf_env E -> uniq E.
-Proof with auto.
-  intros. induction H...
-Qed.
-
-Lemma is_Menv_uniq:
-  forall E E', is_Menv E E' -> uniq E' -> uniq E.
-Proof with auto.
-  intros.
-  induction H...
-  - inversion H0;subst. constructor...
-    rewrite is_Menv_dom with (E:=E')...
-  - inversion H0;subst. constructor...
-    rewrite is_Menv_dom with (E:=E')...
-  - inversion H0;subst. constructor...
-    rewrite is_Menv_dom with (E:=E')...
-Qed.
-
-Theorem completeness: forall E' E A B,
-  is_Menv E E' ->
-  wk_sub E' A B -> forall im,
-  (forall X, 
-     (binds X (M.bind_sub ( im)) E -> posvar Pos  X A B) /\
-     (binds X (M.bind_sub ( (M.flip_im im))) E -> posvar Neg X A B)) ->
-  (exists evs, M.Sub im M.Lt evs E A B) \/ (exists evs, M.Sub im M.Eq evs E A B).
-Proof with auto.
-  intros. generalize dependent E.
-  dependent induction H0;intros...
-  - right. exists M.emp... apply M.Sa_nat...
-    apply is_Menv_wf_env with (E:=E)...
-  - destruct (decide_typ A typ_top).
-    + subst. right. exists M.emp... apply M.Sa_top_eq...
-      apply is_Menv_wf_env with (E:=E)...
-    + left. exists M.emp... apply M.Sa_top_lt...
-      apply is_Menv_wf_env with (E:=E)...
-      apply MWF_WFS with (E':=E)...
-  - right.
-    assert (binds X (M.bind_sub im) E0 \/ binds X (M.bind_sub (M.flip_im im)) E0).
-    { apply is_Menv_case with (E:=E)... }
-    destruct H3.
-    + exists M.emp. apply M.Sa_fvar_pos...
-      eapply is_Menv_wf_env;eassumption.
-    + exists {{ X }}. apply M.Sa_fvar_neg...
-      eapply is_Menv_wf_env;eassumption.
-  
-  - destruct (IHwk_sub1) with (im:=M.flip_im im) (E0:=E0) as [[evs1 IH1]|[evs1 IH1]]...
-    { intros. specialize (H1 X). destruct H1. split;intros.
-      + apply H1 in H2. inversion H2;subst...
-      + destruct im; apply H0 in H2;inversion H2;subst... }
-    + destruct (IHwk_sub2) with (im:=im) (E0:=E0) as [[evs2 IH2]|[evs2 IH2]]...
-      { intros. specialize (H1 X). destruct H1. split;intros.
-        + apply H0 in H2. inversion H2;subst...
-        + destruct im; apply H1 in H2;inversion H2;subst... }
-      * left. exists (evs1 `union` evs2). apply M.Sa_arrow with (cm1:=M.Lt) (cm2:=M.Lt)...
-      * destruct (AtomSetImpl.is_empty evs2) eqn:Eempty.
-        2:{ apply is_not_empty_iff in Eempty. apply not_empty_has in Eempty.
-            destruct Eempty as [X Eempty].
-            pose proof posvar_false _ _ _ _ _ _ IH2 X Eempty.
-            destruct H0.
-            assert (binds X (M.bind_sub im) E0 \/ binds X (M.bind_sub (M.flip_im im)) E0).
-            { apply is_Menv_case with (E:=E)...
-              destruct (M.sub_evs_fv _ _ _ _ _ IH2).
-              rewrite H3 in Eempty.
-              apply wk_sub_to_sam2 in H0_0.
-              apply suba2_regular in H0_0.
-              destruct_hypos. apply WFA_binds with (A:=A2)...
-            }
-            destruct H3.
-            { destruct H1 with (X:=X)... specialize (H4 H3). inversion H4;subst. exfalso. apply H0... }
-            { destruct H1 with (X:=X)... specialize (H5 H3). inversion H5;subst. exfalso. apply H2... }
-        }
-        left. exists (evs1 `union` evs2).
-        apply M.Sa_arrow with (cm1:=M.Lt) (cm2:=M.Eq)... simpl. rewrite Eempty...
-    + destruct (AtomSetImpl.is_empty evs1) eqn:Eempty.
-      2:{ apply is_not_empty_iff in Eempty. apply not_empty_has in Eempty.
-          destruct Eempty as [X Eempty].
-          pose proof posvar_false _ _ _ _ _ _ IH1 X Eempty.
-          destruct H0.
-          assert (binds X (M.bind_sub im) E0 \/ binds X (M.bind_sub (M.flip_im im)) E0).
-          { apply is_Menv_case with (E:=E)...
-            destruct (M.sub_evs_fv _ _ _ _ _ IH1).
-            rewrite H3 in Eempty.
-            apply wk_sub_to_sam2 in H0_.
-            apply suba2_regular in H0_.
-            destruct_hypos. apply WFA_binds with (A:=B1)... }
-          destruct H3.
-          { destruct H1 with (X:=X)... specialize (H4 H3). inversion H4;subst. exfalso. apply H2... destruct im... }
-          { destruct H1 with (X:=X)... specialize (H5 H3). inversion H5;subst. exfalso. apply H0... }
-      }
-      destruct (IHwk_sub2) with (im:=im) (E0:=E0) as [[evs2 IH2]|[evs2 IH2]]...
-      { intros. specialize (H1 X). destruct H1. split;intros.
-        + apply H0 in H2. inversion H2;subst...
-        + destruct im; apply H1 in H2;inversion H2;subst... }
-      * 
-        left. exists (evs1 `union` evs2).
-        apply M.Sa_arrow with (cm1:=M.Eq) (cm2:=M.Lt)... simpl. rewrite Eempty...
-      *
-        (* destruct (AtomSetImpl.is_empty evs2) eqn:Eempty2.
-        2:{ apply is_not_empty_iff in Eempty2. apply not_empty_has in Eempty2.
-            destruct Eempty2 as [X Eempty2].
-            pose proof posvar_false _ _ _ _ _ _ IH2 X Eempty2.
-            destruct H0.
-            assert (binds X (M.bind_sub im) E0 \/ binds X (M.bind_sub (M.flip_im im)) E0).
-            { admit. }
-            destruct H3.
-            { destruct H1 with (X:=X)... specialize (H4 H3). inversion H4;subst. exfalso. apply H0... }
-            { destruct H1 with (X:=X)... specialize (H5 H3). inversion H5;subst. exfalso. apply H2... }
-        } *)
-        right. exists (evs1 `union` evs2).
-        apply M.Sa_arrow with (cm1:=M.Eq) (cm2:=M.Eq)...
-
-(* another discovery:
-  it should also be safe to postpone the equality variable check?
-*)
-
+    (* Top *)
+    simpl. admit.
 
   -
-    pick_fresh X.
-    specialize_x_and_L X L.
-    assert (Hwfe: M.wf_env (X ~ M.bind_sub im ++ E0)).
-    { apply wk_sub_to_sam2 in H.
-      apply suba2_regular in H. destruct_hypos.
-      inversion H;subst... constructor...
-      apply is_Menv_wf_env with (E0:=E0) in H8...
-    }
+    (* arrow *)
+    simpl. apply Sa_arrow with (cm1:=Lt) (cm2:=Lt).
     
-    destruct H0 with (im:=im) (E0:= X ~ M.bind_sub im ++ E0) as [[evs1 IH1]|[evs1 IH1]]...
-    { destruct im; constructor... }
-    { intros. split;intros.
-      + analyze_binds_uniq H4.
-        apply H3 in BindsTac.
-        inversion BindsTac;subst...
-        { destruct H3 with (X:=X0)...
-          pick_fresh Y. specialize_x_and_L Y (union L0 (singleton X0)).
-          rewrite subst_tt_intro with (X:=Y) (T2:=A)...
-          rewrite subst_tt_intro with (X:=Y) (T2:=B)...
-          apply pos_rename_fix... }
-        { apply posvar_self_notin...
-          { pick_fresh Z. specialize_x_and_L Z (union L0 {{X0}})...
-            rewrite subst_tt_intro with (X:=Z)...
-            apply subst_tt_type... }
-          { apply notin_fv_tt_open_aux... }
-        }
-      + analyze_binds_uniq H4.
-        { destruct im; inversion BindsTacVal. }
-        apply H3 in BindsTac.
-        inversion BindsTac;subst...
-        { destruct H3 with (X:=X0)...
-          pick_fresh Y. specialize_x_and_L Y (union L0 (singleton X0)).
-          rewrite subst_tt_intro with (X:=Y) (T2:=A)...
-          rewrite subst_tt_intro with (X:=Y) (T2:=B)...
-          apply pos_rename_fix... }
-        { apply posvar_self_notin...
-          { pick_fresh Z. specialize_x_and_L Z (union L0 {{X0}})...
-            rewrite subst_tt_intro with (X:=Z)...
-            apply subst_tt_type... }
-          { apply notin_fv_tt_open_aux... }
-        }
-    }
-    + (* Lt *)
-      left. exists evs1.
-      apply M.Sa_rec_lt with (L:=L \u {{ X }} \u dom E0)...
-      intros.
-      replace evs1 with (if AtomSetImpl.mem X evs1 then AtomSetImpl.add X0 (remove X evs1) else evs1)...
-      2:{ destruct (AtomSetImpl.mem X evs1) eqn:Eevs...
-          apply mem_iff in Eevs.
-          pose proof posvar_false _ _ _ _ _ _ IH1 X Eevs.
-          destruct H5.
-          exfalso. apply H5... }
-      rewrite_alist (nil ++ X0 ~ M.bind_sub im ++ E0).
-      apply M.sub_replacing_var...
-      { inversion Hwfe;subst... constructor... }
+    (* 
+   
+    TODO: 
+    1) add the second conclusion: flip im ~ subst D and C
+    2) case analysis on cm1 cm2
 
-    + (* Eq *)
-      right.
-      destruct (AtomSetImpl.mem X evs1) eqn:Eevs1.
-      * exists ((remove X evs1) `union` fv_tt A)...
-        apply M.Sa_rec_eq_in with (L:=L \u {{ X }} \u dom E0)...
-        intros.
-        replace (add X0 (remove X evs1)) with (if AtomSetImpl.mem X evs1 then AtomSetImpl.add X0 (remove X evs1) else evs1)...
-        2:{ rewrite Eevs1... }
-        rewrite_alist (nil ++ X0 ~ M.bind_sub im ++ E0).
-        apply M.sub_replacing_var...
-        { inversion Hwfe;subst... constructor... }
-      * exists evs1.
-        apply M.Sa_rec_eq_notin with (L:=L \u {{ X }} \u dom E0)...
-        intros.
-        replace evs1 with (if AtomSetImpl.mem X evs1 then AtomSetImpl.add X0 (remove X evs1) else evs1)... 2:{ rewrite Eevs1... }
-        rewrite_alist (nil ++ X0 ~ M.bind_sub im ++ E0).
-        apply M.sub_replacing_var...
-        { inversion Hwfe;subst... constructor... }
-  - right. apply Msub_refl...
-    + apply is_Menv_wf_env with (E:=E)...
-    + apply wf_type in H0...
-    + apply MWF_WFS with (E':=E)...
-Qed.
+    *)
 
-Theorem completeness_final: forall A B,
-  wk_sub nil A B -> forall im,
-  (exists evs, M.Sub im M.Lt evs nil A B) \/ 
-  (exists evs, M.Sub im M.Eq evs nil A B).
+    admit. admit. admit.
+  
+  -
+    (* mu *)
+    simpl. apply Sa_rec_lt with (L:=L \u fv_tt C \u fv_tt D \u fv_tt A1 \u fv_tt A2 \u {{X}}).
+    intros. specialize_x_and_L X0 L.
+    rewrite subst_tt_open_tt_var...
+    2:{ admit. }
+    rewrite subst_tt_open_tt_var...
+    2:{ admit. }
+    rewrite <- app_assoc.
+    apply H2... admit.
+  -
+     (* proper *)
+     apply Sa_evs_proper with (evs:=evs)...
+Admitted.
+
+Lemma unfolding_lemma :
+  forall E A B evs,
+    Sub Pos Lt evs E (typ_mu A) (typ_mu B) ->
+    Sub Pos Lt evs E (open_tt A (typ_mu A)) (open_tt B (typ_mu B)).
 Proof with auto.
   intros.
-  apply completeness with (E:=nil) (im:=im) in H...
-  { constructor. }
-  { intros. split;intros;inversion H0. }
+  assert (Hq:=H).
+  dependent induction H.
+  +
+    pick fresh X. specialize_x_and_L X L.
+    rewrite_alist (nil ++ E).
+    rewrite subst_tt_intro with (X:=X)...
+    rewrite subst_tt_intro with (X:=X) (T2:=B)...
+    subst.
+    apply sub_regular in Hq.
+    destruct_hypos.
+    apply generalized_unfolding_lemma...
+  +
+    apply Sa_evs_proper with (evs:=evs)...
 Qed.
